theories/Universe.v
@@ -1,12 +1,35 @@
+Require Import Coqlib.
 Require Export ZArith.
 Require Export String.
+
+Set Implicit Arguments.
+
+(************ temporary buffer before putting it in Coqlib ***********)
+(************ temporary buffer before putting it in Coqlib ***********)
+(************ temporary buffer before putting it in Coqlib ***********)
+
+Class Dec (A: Type) := dec: forall (a0 a1: A), { a0 = a1 } + { a0 <> a1 }.
+
+Global Program Instance positive_Dec: Dec positive. Next Obligation. decide equality. Defined.
+Global Program Instance string_Dec: Dec String.string. Next Obligation. apply String.string_dec. Defined.
+Global Program Instance nat_Dec: Dec nat. Next Obligation. apply Nat.eq_dec. Defined.
+Global Program Instance Z_Dec: Dec Z. Next Obligation. apply Z.eq_dec. Defined.
+
+Definition update K `{Dec K} V (f: K -> V) (k: K) (v: V): K -> V :=
+  fun _k => if dec k _k then v else f _k.
+
+(************ temporary buffer before putting it in Coqlib ***********)
+(************ temporary buffer before putting it in Coqlib ***********)
+(************ temporary buffer before putting it in Coqlib ***********)
+
+
 
 Notation block := nat (only parsing).
 
 Inductive val: Type :=
 | Vint (n: Z): val
 | Vptr (blk: block) (ofs: Z): val
-| Vundef
+(* | Vundef *)
 .
 
 Notation fname := string (only parsing).
@@ -22,7 +45,23 @@ Inductive event: Type :=
 
 Module Mem.
 
-  Definition t: Type := block -> option (Z -> val).
+  (* Definition t: Type := block -> option (Z -> val). *)
+  Record t: Type := mk {
+    contents: block -> Z -> option val;
+    nextblock: block;
+    (*** nextblock_noaccess ? ***)
+  }
+  .
+
+  Definition empty: t := mk (fun _ _ => None) 0.
+
+  Definition alloc (m0: Mem.t) (sz: Z): (block * Mem.t) :=
+    ((m0.(nextblock)),
+     Mem.mk (update (m0.(contents)) (m0.(nextblock))
+                    (fun ofs => if (0 <=? ofs) && (ofs <? sz) then Some (Vint 0) else None))
+            (S m0.(nextblock))
+    )
+  .
 
 End Mem.
 
