theories/Sem.v
@@ -21,59 +21,53 @@ Section INTERP.
   Context `{GRA: GRA.t}.
   Variable ms: ModSem.t.
 
-  Let itr0: callE ~> itree (callE +' mdE +' fnE +' eventE) :=
+  Let itr0: callE ~> itree Es :=
     fun _ ce =>
-      trigger FPush;;
+      trigger PushFrame;;
       rv <- (ms.(ModSem.sem) ce);;
-      trigger FPop;;
+      trigger PopFrame;;
       Ret rv
   .
-  Let itr1: itree (mdE +' fnE +' eventE) val := (mrec itr0) _ (Call "main" nil).
+  Let itr1: itree (rE +' eventE) val := (mrec itr0) _ (Call "main" nil).
 
 
 
-  Definition md_state: Type := mname -> GRA.
-  Definition handle_mdE `{eventE -< E}: mdE ~> stateT md_state (itree E) :=
-    fun _ e st0 =>
-      match e with
-      | MPut mn gr =>
-        guarantee(RA.updatable (st0 mn) gr);;
-        Ret (update st0 mn gr, tt)
-      | MGet mn => Ret (st0, st0 mn)
-      end.
-  Definition interp_mdE `{eventE -< E}: itree (mdE +' E) ~> stateT md_state (itree E) :=
-    State.interp_state (case_ handle_mdE State.pure_state).
-  Definition initial_md_state: md_state :=
-    fun mn => match List.find (fun mnr => dec mn (fst mnr)) ms.(ModSem.initial_ld) with
-              | Some r => snd r
-              | None => URA.unit
-              end.
-  Let itr2: itree (fnE +' eventE) val := snd <$> (interp_mdE itr1) initial_md_state.
-
-
-
-  Definition fn_state: Type := list GRA.
-  Definition handle_fnE `{eventE -< E}: fnE ~> stateT fn_state (itree E) :=
-    fun _ e st0 =>
-      match e with
-      | FPut gr =>
-        match st0 with
-        | nil => triggerNB
-        | hd :: tl =>
-          guarantee(RA.updatable hd gr);;
-          Ret (gr :: tl, tt)
+  Definition r_state: Type := ((mname -> GRA) * list GRA).
+  Definition handle_rE `{eventE -< E}: rE ~> stateT r_state (itree E) :=
+    fun _ e '(mrs, frs) =>
+      match frs with
+      | hd :: tl =>
+        match e with
+        | Put mn mr fr =>
+          guarantee(URA.updatable (URA.add (mrs mn) hd) (URA.add mr fr));;
+          Ret (((update mrs mn mr), fr :: tl), tt)
+        | MGet mn => Ret ((mrs, frs), mrs mn)
+        | FGet => Ret ((mrs, frs), hd)
+        | Forge fr => Ret ((mrs, (URA.add hd fr) :: tl), tt)
+        | Discard fr =>
+          rest <- trigger (Choose _);;
+          guarantee(hd = URA.add fr rest);;
+          Ret ((mrs, rest :: tl), tt)
+        | CheckWf mn =>
+          assume(URA.wf (URA.add (mrs mn) hd));;
+          Ret ((mrs, frs), tt)
+        | PushFrame =>
+          Ret ((mrs, URA.unit :: frs), tt)
+        | PopFrame =>
+          Ret ((mrs, tl), tt)
         end
-      | FGet =>
-        hd <- (hd_error st0)﹗ ;;
-        Ret (st0, hd)
-      | FPush =>
-        Ret (URA.unit :: st0, tt)
-      | FPop =>
-        Ret (tl st0, tt)
+      | _ => triggerNB
       end.
-  Definition interp_fnE `{eventE -< E}: itree (fnE +' E) ~> stateT fn_state (itree E) :=
-    State.interp_state (case_ handle_fnE State.pure_state).
-  Let itr3: itree (eventE) val := snd <$> (interp_fnE itr2) nil.
+  Definition interp_rE `{eventE -< E}: itree (rE +' E) ~> stateT r_state (itree E) :=
+    State.interp_state (case_ handle_rE State.pure_state).
+  Definition initial_r_state: r_state :=
+    (fun mn => match List.find (fun mnr => dec mn (fst mnr)) ms.(ModSem.initial_ld) with
+               | Some r => snd r
+               | None => URA.unit
+               end, []).
+  Let itr2: itree (eventE) val := snd <$> (interp_rE itr1) initial_r_state.
+
+
 
   Let state: Type := itree eventE val.
 
@@ -110,7 +104,7 @@ Section INTERP.
   Program Definition interp: semantics := {|
     STS.state := state;
     STS.step := step;
-    STS.initial_state := itr3;
+    STS.initial_state := itr2;
     STS.state_sort := state_sort;
   |}
   .
